More work toward finishing exercises

SearchTree.v
@@ -5,9 +5,13 @@
 (* IMPORTS *)
 Require Import ZArith Permutation Omega List Classical_sets.
 Require Import FunctionalExtensionality.
+Require Export CpdtTactics.
 Axiom prop_ext: ClassicalFacts.prop_extensionality.
 Implicit Arguments prop_ext.
 Open Scope Z.
+
+Ltac inv H := inversion H; subst; clear H.
+Ltac appinv t H := apply t in H; inv H.
 
 (* A FEW LEMMAS ABOUT SET UNION, ET CETERA *)
 Arguments In {U} A x.
@@ -27,25 +31,50 @@ Lemma In_Union_iff:
  forall U (B C: Ensemble U) x,
   In (Union B C) x <-> (In B x \/ In C x).
 Proof.
-(* FILL IN HERE *) Admitted.
+  intros. split.
+    intros. inversion H.
+      left. apply H0.
+      right. apply H0.
+    intros. inversion H.
+      apply Union_introl. apply H0.
+      apply Union_intror. apply H0.
+Qed.
 
 Lemma Union_Empty_set_l: forall U (B: Ensemble U),
   Union Empty_set B = B.
 Proof.
-intros. extensionality x. apply prop_ext.
-(* FILL IN HERE *) Admitted.
+  intros. extensionality x. apply prop_ext.
+  split; intros.
+    inversion H; subst. apply Empty_set_ind. apply H0. apply H0.
+    apply Union_intror. apply H.
+Qed.
 
 Lemma Union_sym:
  forall {U} (B C: Ensemble U), Union B C = Union C B.
 Proof.
   intros. extensionality x. apply prop_ext.
-(* FILL IN HERE *) Admitted.
+  split; intros; inversion H; subst.
+  - apply Union_intror. apply H0.
+  - apply Union_introl. apply H0.
+  - apply Union_intror. apply H0.
+  - apply Union_introl. apply H0.
+Qed.
 
 Lemma Union_assoc:
   forall {U} (A B C: Ensemble U),
    Union A (Union B C) = Union (Union A B) C.
 Proof.
-(* FILL IN HERE *) Admitted.
+  intros. extensionality x. apply prop_ext.
+  split; intros; inversion H; subst.
+  - apply Union_introl. apply Union_introl. apply H0.
+  - inversion H0; subst.
+    apply Union_introl. apply Union_intror. apply H1.
+    apply Union_intror. apply H1.
+  - inversion H0; subst.
+    apply Union_introl. apply H1.
+    apply Union_intror. apply Union_introl. apply H1.
+  - apply Union_intror. apply Union_intror. apply H0.
+Qed.
 
 (*  PROGRAM FOR BINARY SEARCH TREES *)
 
@@ -71,26 +100,92 @@ Fixpoint insert (x: Z) (s: tree) :=
 
 (* SPECIFICATIONS AND PROOF *)
 
+Inductive OccursTree : Z -> tree -> Prop :=
+  | occ_root n a b : OccursTree n (T a n b)
+  | occ_left n a b : forall p, OccursTree n a -> OccursTree n (T a p b)
+  | occ_right n a b : forall p, OccursTree n b -> OccursTree n (T a p b).
+
+Hint Constructors OccursTree.
+
+Definition all_lt (n : Z) (t : tree) := forall x, OccursTree x t -> x < n.
+Definition all_gt (n : Z) (t : tree) := forall x, OccursTree x t -> x > n.
+
+Hint Extern 1 (all_lt _ _) => unfold all_lt; intros.
+Hint Extern 1 (all_gt _ _) => unfold all_gt; intros.
 
 Inductive SearchTree: tree -> Prop :=
 (* Getting this right is the most important part of the work,
  *   and it's not completely obvious.
  *)
-(* FILL IN HERE *).
+  | bst_empty : SearchTree E
+  | bst_node n a b : SearchTree a -> SearchTree b
+                       -> all_lt n a -> all_gt n b
+                       -> SearchTree (T a n b).
 
-Inductive Contents:  Ensemble Z -> tree -> Prop :=
+Hint Constructors SearchTree.
+
+Inductive Contents: Ensemble Z -> tree -> Prop :=
 | Ct_E: Contents Empty_set E
-(* FILL IN HERE *).
+| Ct_U A B l x r: Contents A l -> Contents B r
+    -> Contents (Union A B) (T l x r).
 
-
+Theorem member_or: forall k z t1 t2,
+  member k (T t1 z t2) = true -> member k t1 = true \/ member k t2 = true \/ k = z.
+Proof.
+  intros. inversion H.
+  destruct (k <? z) eqn:Heqe;
+    [ apply Z.ltb_lt in Heqe | apply Z.ltb_nlt in Heqe ].
+  - left. reflexivity.
+  - destruct (z <? k) eqn:Heqe2;
+      [ apply Z.ltb_lt in Heqe2 | apply Z.ltb_nlt in Heqe2 ].
+    right. left. reflexivity.
+    inversion H. crush.
+Qed.
 
 Theorem member_spec:
+  forall k t, SearchTree t -> (member k t = true <-> OccursTree k t).
+Proof.
+  intros. split; induction t; intros; simpl.
+  - crush.
+  - inv H. appinv member_or H0; crush.
+  - inversion H0.
+  - destruct (k <? z) eqn:Heqe;
+      [ apply Z.ltb_lt in Heqe | apply Z.ltb_nlt in Heqe ].
+    + inv H. inv H0; crush.
+      apply H7 in H2. omega.
+    + destruct (z <? k) eqn:Heqe2;
+        [ apply Z.ltb_lt in Heqe2 | apply Z.ltb_nlt in Heqe2 ].
+      * inv H. inv H0; crush.
+      * crush.
+Qed.
+
+Theorem member_spec_orig:
   forall k cts t,
     SearchTree t ->
     Contents cts t ->
     (In cts k <->  member k t = true).
 Proof.
-(* FILL IN HERE *) Admitted.
+  intros. split; intros; induction t; crush.
+    inv H. inv H0. inv H1.
+  destruct (k <? z) eqn:Heqe;
+    [ apply Z.ltb_lt in Heqe | apply Z.ltb_nlt in Heqe ].
+    apply IHt1. inv H. crush.
+Abort.
+
+Theorem insert_occurstree:
+  forall k x t, OccursTree x t -> OccursTree x (insert k t).
+Proof.
+  intros.
+  induction t; intros. crush.
+  simpl. destruct (k <? z) eqn:Heqe;
+      [ apply Z.ltb_lt in Heqe | apply Z.ltb_nlt in Heqe ].
+    inv H; crush.
+  destruct (z <? k) eqn:Heqe2;
+      [ apply Z.ltb_lt in Heqe2 | apply Z.ltb_nlt in Heqe2 ].
+    inv H; crush.
+  assert (k = z). omega.
+  rewrite H0. crush.
+Qed.
 
 Theorem insert_contents:
  forall k t cts,
@@ -98,10 +193,45 @@ Theorem insert_contents:
     Contents cts t ->
     Contents (Union (Singleton k) cts) (insert k t).
 Proof.
-(* FILL IN HERE *) Admitted.
+  intros.
+  generalize dependent k.
+  induction t.
+    constructor; crush.
+    inv H0. inv H.
+Abort.
 
 Theorem insert_searchtree:
-  forall k t,
-   SearchTree t -> SearchTree (insert k t).
+  forall k t, SearchTree t -> SearchTree (insert k t).
 Proof.
-(* FILL IN HERE *) Admitted.
+  intros.
+  induction t; intros; crush.
+    inv H; crush.
+    constructor; crush; simpl.
+      unfold all_lt. intros. inv H.
+    unfold all_gt. intros. inv H.
+  inv H; crush.
+  destruct (k <? z) eqn:Heqe;
+    [ apply Z.ltb_lt in Heqe | apply Z.ltb_nlt in Heqe ].
+    constructor; crush.
+    unfold all_lt. intros.
+    unfold all_lt in *.
+    unfold all_gt in *.
+    apply H5.
+    apply member_spec. auto.
+    admit.
+  destruct (z <? k) eqn:Heqe2;
+    [ apply Z.ltb_lt in Heqe2 | apply Z.ltb_nlt in Heqe2 ].
+    constructor; crush.
+    unfold all_gt. intros.
+    unfold all_lt in *.
+    unfold all_gt in *.
+    apply H6.
+    apply member_spec. auto.
+    admit.
+  constructor; crush.
+  unfold all_lt in *.
+  unfold all_gt in *.
+  apply Znot_lt_ge in Heqe.
+  apply Znot_lt_ge in Heqe2.
+  intros.
+Abort.
